\documentclass{article}
\usepackage{amsmath}
\usepackage{amssymb}
\usepackage{graphicx}
\usepackage{tikz}
\usepackage{pgfplots}
\usepackage{float}
\usepackage{subcaption}
\usepackage{geometry}

\geometry{a4paper, margin=1in}

% Define example environment
\newenvironment{example}[1]{
    \begin{trivlist}
    \item[\textbf{Example:}] #1
    \vspace{0.5em}
}{
    \end{trivlist}
    \vspace{1em}
}

\pgfplotsset{compat=1.18}
\usetikzlibrary{patterns,decorations.pathreplacing}

\title{Lecture 5 Examples}
\author{Signals and Systems Course}
\date{}

\begin{document}

\maketitle

\begin{example}[1. Continuous-Time Convolution: Exponential and Unit Step]
\textbf{Problem:}
Find the convolution $y(t) = x(t) * h(t)$ where:
\begin{align}
    x(t) &= u(t) \quad \text{(unit step function)} \\
    h(t) &= e^{-at} u(t), \quad a > 0 \quad \text{(exponential impulse response)}
\end{align}

\begin{figure}[H]
    \centering
    \begin{minipage}{0.45\textwidth}
        \centering
        \resizebox{!}{5cm}{ \input{figures/lec05_examples/unit_step_ct.tex}}
        \caption{Input signal $x(t) = u(t)$}
    \end{minipage}\hfill
    \begin{minipage}{0.45\textwidth}
        \centering
      \resizebox{!}{5cm}{   \input{figures/lec05_examples/exponential_impulse.tex}}
        \caption{Impulse response $h(t) = e^{-at} u(t)$}
    \end{minipage}
\end{figure}

\textbf{Solution:}

$$y(t) = \int_{0}^{t} e^{-a(t-\tau)} d\tau = e^{-at} \int_{0}^{t} e^{a\tau} d\tau = \frac{1 - e^{-at}}{a}$$

For $t < 0$: $y(t) = 0$

\textbf{Answer:}
$$y(t) = \frac{1 - e^{-at}}{a} u(t)$$

\begin{figure}[H]
    \centering
    \input{figures/lec05_examples/step_response.tex}
    \caption{Step response $y(t) = x(t) * h(t)$}
\end{figure}
\end{example}

\vspace{0.5em}
\hrule
\vspace{0.5em}

\begin{example}[2. Convolution of Two-Sided and One-Sided Signals]
\textbf{Problem:}
Find the convolution $y(t) = x(t) * h(t)$ where:
\begin{align}
    x(t) &= e^{-|t|} \quad \text{(two-sided exponential)} \\
    h(t) &= u(t) \quad \text{(unit step function)}
\end{align}

\begin{figure}[H]
    \centering
    \begin{minipage}{0.45\textwidth}
        \centering
        \resizebox{!}{5cm}{\input{figures/lec05_examples/two_sided_exponential.tex}}
        \caption{Input signal $x(t) = e^{-|t|}$}
    \end{minipage}\hfill
    \begin{minipage}{0.45\textwidth}
        \centering
       \resizebox{!}{5cm}{ \input{figures/lec05_examples/unit_step_ct2.tex}}
        \caption{Impulse response $h(t) = u(t)$}
    \end{minipage}
\end{figure}

\textbf{Solution:}

$$y(t) = \int_{-\infty}^{t} e^{-|\tau|} d\tau$$

\textbf{Case 1:} $t < 0$
$$y(t) = \int_{-\infty}^{t} e^{\tau} d\tau = e^{t}$$

\textbf{Case 2:} $t \geq 0$
$$y(t) = \int_{-\infty}^{0} e^{\tau} d\tau + \int_{0}^{t} e^{-\tau} d\tau = 1 + (1 - e^{-t}) = 2 - e^{-t}$$

\textbf{Answer:}
$$y(t) = \begin{cases}
    e^{t} & \text{for } t < 0 \\
    2 - e^{-t} & \text{for } t \geq 0
\end{cases}$$

\begin{figure}[H]
    \centering
    \input{figures/lec05_examples/two_sided_convolution.tex}
    \caption{Convolution result $y(t) = x(t) * h(t)$}
\end{figure}
\end{example}

\vspace{0.5em}
\hrule
\vspace{0.5em}

\begin{example}[3. Convolution with Rectangular Pulse]
\textbf{Problem:}
Find the convolution $y(t) = x(t) * h(t)$ where:
\begin{align}
    x(t) &= e^{-at} u(t), \quad a > 0 \\
    h(t) &= \begin{cases}
        1 & \text{for } 0 \leq t \leq T \\
        0 & \text{otherwise}
    \end{cases}
\end{align}

\begin{figure}[H]
    \centering
    \begin{minipage}{0.45\textwidth}
        \centering
         \resizebox{!}{5cm}{\input{figures/lec05_examples/exponential_input.tex}}
        \caption{Input signal $x(t) = e^{-at} u(t)$}
    \end{minipage}\hfill
    \begin{minipage}{0.45\textwidth}
        \centering
        \resizebox{!}{5cm}{ \input{figures/lec05_examples/rectangular_pulse.tex}}
        \caption{Impulse response $h(t)$ (rectangular pulse)}
    \end{minipage}
\end{figure}

\textbf{Solution:}

$$y(t) = \int_{\max(0, t-T)}^{t} e^{-a\tau} d\tau$$

\textbf{Case 1:} $t < 0$ â†’ $y(t) = 0$

\textbf{Case 2:} $0 \leq t \leq T$
$$y(t) = \int_{0}^{t} e^{-a\tau} d\tau = \frac{1 - e^{-at}}{a}$$

\textbf{Case 3:} $t > T$
$$y(t) = \int_{t-T}^{t} e^{-a\tau} d\tau = \frac{e^{-a(t-T)} - e^{-at}}{a} = \frac{e^{-at}(e^{aT} - 1)}{a}$$

\textbf{Answer:}
$$y(t) = \begin{cases}
    0 & \text{for } t < 0 \\
    \frac{1 - e^{-at}}{a} & \text{for } 0 \leq t \leq T \\
    \frac{e^{-at}(e^{aT} - 1)}{a} & \text{for } t > T
\end{cases}$$

\begin{figure}[H]
    \centering
    \input{figures/lec05_examples/rectangular_convolution.tex}
    \caption{Convolution result $y(t) = x(t) * h(t)$}
\end{figure}
\end{example}

\vspace{0.5em}
\hrule
\vspace{0.5em}

\begin{example}[4. Convolution with Impulse Train]
\textbf{Problem:}
Find $y(t) = x(t) * h(t)$ where $x(t) = \cos(\omega_0 t)$ and $h(t) = \sum_{n=-\infty}^{\infty} \delta(t - nT)$.

\textbf{Solution:}
Using sifting property: $y(t) = \sum_{n=-\infty}^{\infty} \cos(\omega_0 (t - nT))$

Using the identity $\cos(A-B) = \cos A \cos B + \sin A \sin B$:
$$y(t) = \sum_{n=-\infty}^{\infty} [\cos(\omega_0 t)\cos(\omega_0 nT) + \sin(\omega_0 t)\sin(\omega_0 nT)]$$

$$= \cos(\omega_0 t) \sum_{n=-\infty}^{\infty} \cos(\omega_0 nT) + \sin(\omega_0 t) \sum_{n=-\infty}^{\infty} \sin(\omega_0 nT)$$

Since $\sum_{n=-\infty}^{\infty} \sin(\omega_0 nT) = 0$ (odd symmetry):
$$y(t) = \cos(\omega_0 t) \sum_{n=-\infty}^{\infty} \cos(\omega_0 nT)$$

\textbf{Answer:} $y(t) = \cos(\omega_0 t) \sum_{n=-\infty}^{\infty} \cos(\omega_0 nT)$
\end{example}

\end{document}